LeanNanoLlvm/Refinement/Test.lean
@@ -43,6 +43,12 @@ private theorem intw_add_zero (x : Semantics.IntW 8) :
   | ofOption o =>
     cases o <;> simp
 
+private theorem intw_add_zero_generic {w : Nat} (x : Semantics.IntW w) :
+    (do let y ← x; PoisonOr.value (y + (0 : BitVec w))) = x := by
+  cases x with
+  | ofOption o =>
+    cases o <;> simp
+
 
 theorem ret_add_x_0_refines_ret_x : retAddX0Def ⊑ retXDef := by
   intro args undefs retval hwfAdd hwfRet hsig hargs h
@@ -59,6 +65,47 @@ theorem ret_add_x_0_refines_ret_x : retAddX0Def ⊑ retXDef := by
           simp [retAddX0Def, simp_llvm, simp_wellform, simp_llvm_option] at *
       | cons arg' rest' =>
           simp [Semantics.Definition.ArgValuesWellFormed, retAddX0Def] at hargs
+
+open scoped LeanNanoLlvm.AST.Syntax in
+def retAddX0Poly : @AST.Definition 1 := [llvm-1-definition|
+  define i$0 @f(i$0 %x) {
+  entry:
+    %x = add i$0 %x, 0
+    ret i$0 %x
+  }
+]
+
+open scoped LeanNanoLlvm.AST.Syntax in
+def retXPoly : @AST.Definition 1 := [llvm-1-definition|
+  define i$0 @f(i$0 %x) {
+  entry:
+    ret i$0 %x
+  }
+]
+
+abbrev singletonWidths (w : Nat) : List.Vector Nat 1 := ⟨[w], by simp⟩
+
+theorem ret_add_x_0_refines_ret_x_generic (w : Nat) :
+    retAddX0Poly.instantiateWidths (singletonWidths w) ⊑ retXPoly.instantiateWidths (singletonWidths w) := by
+  intro args undefs retval hwfAdd hwfRet hsig hargs h
+  cases args with
+  | nil =>
+      simp [Semantics.Definition.ArgValuesWellFormed, retAddX0Poly, singletonWidths] at hargs
+  | cons arg rest =>
+      cases rest with
+      | nil =>
+          cases arg <;> simp [Semantics.Definition.ArgValuesWellFormed,
+            Semantics.RegisterValue.WellFormedFor, retAddX0Poly, singletonWidths] at hargs
+          rename_i w' v
+          subst hargs
+          simp [singletonWidths, retAddX0Poly, retXPoly, simp_llvm, simp_wellform, simp_llvm_option] at h ⊢
+          change Except.ok (RegisterValue.bv w v) = Except.ok retval at h
+          change Except.ok (RegisterValue.bv w (do let x ← v; PoisonOr.value (x + (0 : BitVec w)))) =
+            Except.ok retval
+          rw [intw_add_zero_generic v]
+          exact h
+      | cons arg' rest' =>
+          simp [Semantics.Definition.ArgValuesWellFormed, retAddX0Poly, singletonWidths] at hargs
 
 
 end LeanNanoLlvm.Refinement
